Refactoring

Definitions.v
@@ -1,8 +1,405 @@
-From Elo Require Export ValidAddresses.
-From Elo Require Export WellTypedTerm.
-From Elo Require Export CTR.
-From Elo Require Export Access.
-From Elo Require Export UnsafeAccess.
-From Elo Require Export SafeSpawns.
-From Elo Require Export SMS.
+From Elo Require Import Core.
+
+(* ------------------------------------------------------------------------- *)
+(* has-address                                                               *)
+(* ------------------------------------------------------------------------- *)
+
+Reserved Notation "t 'has_address' ad" (at level 80, no associativity).
+
+Inductive has_ad : addr -> tm -> Prop :=
+  | ha_ref : forall ad T,
+    <{&ad :: T}> has_address ad
+
+  | ha_new : forall ad t T,
+    has_ad ad t ->
+    has_ad ad <{new T t}>
+
+  | ha_load : forall ad t,
+    has_ad ad t ->
+    has_ad ad <{*t}>
+
+  | ha_asg1 : forall ad t1 t2,
+    has_ad ad t1 ->
+    has_ad ad <{t1 = t2}>
+
+  | ha_asg2 : forall ad t1 t2,
+    has_ad ad t2 ->
+    has_ad ad <{t1 = t2}>
+
+  | ha_seq1 : forall ad t1 t2,
+    has_ad ad t1 ->
+    has_ad ad <{t1; t2}>
+
+  | ha_seq2 : forall ad t1 t2,
+    has_ad ad t2 ->
+    has_ad ad <{t1; t2}>
+
+  | ha_call1 : forall ad t1 t2,
+    has_ad ad t1 ->
+    has_ad ad <{call t1 t2}>
+
+  | ha_call2 : forall ad t1 t2,
+    has_ad ad t2 ->
+    has_ad ad <{call t1 t2}>
+
+  | ha_fun : forall ad x T t,
+    has_ad ad t ->
+    has_ad ad <{fn x T t}>
+
+  | ha_spawn : forall ad t,
+    has_ad ad t ->
+    has_ad ad <{spawn t}>
+
+  where "t 'has_address' ad" := (has_ad ad t).
+
+(* ------------------------------------------------------------------------- *)
+(* valid-addresses                                                           *)
+(* ------------------------------------------------------------------------- *)
+
+(* The addresses are valid if they are within the bounds of the memory. *)
+Definition valid_addresses (m : mem) (t : tm) :=
+  forall ad, t has_address ad -> ad < #m.
+
+(* ------------------------------------------------------------------------- *)
+(* well-typed-term                                                           *)
+(* ------------------------------------------------------------------------- *)
+
+Definition well_typed_term (t : tm) :=
+  exists T, empty |-- t is T.
+
+(* ------------------------------------------------------------------------- *)
+(* consistently-typed-references                                             *)
+(* ------------------------------------------------------------------------- *)
+
+Inductive consistently_typed_references (m : mem) : tm -> Prop :=
+  | ctr_unit :
+    consistently_typed_references m <{unit}> 
+
+  | ctr_num : forall n,
+    consistently_typed_references m <{N n}>
+
+  | ctr_refM : forall T ad,
+    empty |-- m[ad].tm is T ->
+    m[ad].typ = <{{ &T }}> ->
+    consistently_typed_references m <{&ad :: &T}>
+
+  | ctr_refI : forall T ad,
+    empty |-- m[ad].tm is <{{ Immut T }}> ->
+    m[ad].typ = <{{ i&T }}> ->
+    consistently_typed_references m <{&ad :: i&T}>
+
+  | ctr_new : forall T t,
+    consistently_typed_references m t ->
+    consistently_typed_references m <{new T t}> 
+
+  | ctr_load : forall t,
+    consistently_typed_references m t ->
+    consistently_typed_references m <{*t}> 
+
+  | ctr_asg : forall t1 t2,
+    consistently_typed_references m t1 ->
+    consistently_typed_references m t2 ->
+    consistently_typed_references m <{t1 = t2}> 
+
+  | ctr_var : forall x,
+    consistently_typed_references m <{var x}>
+
+  | ctr_fun : forall x Tx t,
+    consistently_typed_references m t ->
+    consistently_typed_references m <{fn x Tx t}>
+
+  | ctr_call : forall t1 t2,
+    consistently_typed_references m t1 ->
+    consistently_typed_references m t2 ->
+    consistently_typed_references m <{call t1 t2}> 
+
+  | ctr_seq : forall t1 t2,
+    consistently_typed_references m t1 ->
+    consistently_typed_references m t2 ->
+    consistently_typed_references m <{t1; t2}>
+
+  | ctr_spawn : forall t,
+    consistently_typed_references m t ->
+    consistently_typed_references m <{spawn t}>
+  .
+
+(* ------------------------------------------------------------------------- *)
+(* access                                                                    *)
+(* ------------------------------------------------------------------------- *)
+
+(*
+  A term has access to an address if it refers to the address directly or 
+  indirectly.
+  
+  Ignores <spawn> blocks.
+*)
+Inductive access (ad : addr) (m : mem) : tm -> Prop :=
+  | acc_mem : forall ad' T,
+    ad <> ad' ->
+    access ad m m[ad'].tm ->
+    access ad m <{&ad' :: T}>
+
+  | acc_ref : forall T,
+    access ad m <{&ad :: T}>
+
+  | acc_new : forall T t,
+    access ad m t ->
+    access ad m <{new T t}>
+
+  | acc_load : forall t,
+    access ad m t ->
+    access ad m <{*t}>
+
+  | acc_asg1 : forall t1 t2,
+    access ad m t1 ->
+    access ad m <{t1 = t2}>
+
+  | acc_asg2 : forall t1 t2,
+    access ad m t2 ->
+    access ad m <{t1 = t2}>
+
+  | acc_fun : forall x Tx t,
+    access ad m t ->
+    access ad m <{fn x Tx t}>
+
+  | acc_call1 : forall t1 t2,
+    access ad m t1 ->
+    access ad m <{call t1 t2}>
+
+  | acc_call2 : forall t1 t2,
+    access ad m t2 ->
+    access ad m <{call t1 t2}>
+
+  | acc_seq1 : forall t1 t2,
+    access ad m t1 ->
+    access ad m <{t1; t2}>
+
+  | acc_seq2 : forall t1 t2,
+    access ad m t2 ->
+    access ad m <{t1; t2}>
+  .
+
+(* ------------------------------------------------------------------------- *)
+(* valid-accesses                                                            *)
+(* ------------------------------------------------------------------------- *)
+
+(* TODO *)
+Definition valid_accesses (m : mem) (t : tm) :=
+  forall ad, access ad m t -> ad < #m.
+
+(* ------------------------------------------------------------------------- *)
+(* unsafe-access                                                             *)
+(* ------------------------------------------------------------------------- *)
+
+(* There is a mutable pointer to <ad> in the term. *)
+Inductive unsafe_access (ad : addr) (m : mem) : tm  -> Prop :=
+  | uacc_mem : forall ad' T,
+    ad <> ad' ->
+    unsafe_access ad m (m[ad'].tm) ->
+    unsafe_access ad m <{&ad' :: &T}>
+
+  | uacc_ref : forall T,
+    unsafe_access ad m <{&ad :: &T}>
+
+  | uacc_new : forall T t,
+    unsafe_access ad m t ->
+    unsafe_access ad m <{new T t}>
+
+  | uacc_load : forall t,
+    unsafe_access ad m t ->
+    unsafe_access ad m <{*t}>
+
+  | uacc_asg1 : forall t1 t2,
+    unsafe_access ad m t1 ->
+    unsafe_access ad m <{t1 = t2}>
+
+  | uacc_asg2 : forall t1 t2,
+    unsafe_access ad m t2 ->
+    unsafe_access ad m <{t1 = t2}>
+
+  | uacc_fun : forall x Tx t,
+    unsafe_access ad m t ->
+    unsafe_access ad m <{fn x Tx t}>
+
+  | uacc_call1 : forall t1 t2,
+    unsafe_access ad m t1 ->
+    unsafe_access ad m <{call t1 t2}>
+
+  | uacc_call2 : forall t1 t2,
+    unsafe_access ad m t2 ->
+    unsafe_access ad m <{call t1 t2}>
+
+  | uacc_seq1 : forall t1 t2,
+    unsafe_access ad m t1 ->
+    unsafe_access ad m <{t1; t2}>
+
+  | uacc_seq2 : forall t1 t2,
+    unsafe_access ad m t2 ->
+    unsafe_access ad m <{t1; t2}>
+  .
+
+(* ------------------------------------------------------------------------- *)
+(* safe-access                                                               *)
+(* ------------------------------------------------------------------------- *)
+
+Definition safe_access ad m t := access ad m t /\ ~ unsafe_access ad m t.
+
+(* ------------------------------------------------------------------------- *)
+(* no-mut                                                                    *)
+(* ------------------------------------------------------------------------- *)
+
+(* A term is no-mut if it has no mutable references. *)
+Inductive no_mut : tm -> Prop :=
+  | nomut_unit :
+    no_mut <{unit}>
+
+  | nomut_num : forall n,
+    no_mut <{N n}>
+
+  | nomut_ref : forall ad T,
+    no_mut <{&ad :: i&T}>
+
+  | nomut_new : forall T t,
+    no_mut t ->
+    no_mut <{new T t}>
+
+  | nomut_load : forall t,
+    no_mut t ->
+    no_mut <{*t}>
+
+  | nomut_asg : forall t1 t2,
+    no_mut t1 ->
+    no_mut t2 ->
+    no_mut <{t1 = t2}>
+
+  | nomut_var : forall x,
+    no_mut <{var x}>
+
+  | nomut_fun : forall x Tx t,
+    no_mut t ->
+    no_mut <{fn x Tx t}>
+
+  | nomut_call : forall t1 t2,
+    no_mut t1 ->
+    no_mut t2 ->
+    no_mut <{call t1 t2}>
+
+  | nomut_seq : forall t1 t2,
+    no_mut t1 ->
+    no_mut t2 ->
+    no_mut <{t1; t2}>
+
+  | nomut_spawn : forall t,
+    no_mut t ->
+    no_mut <{spawn t}>
+  .
+
+(* ------------------------------------------------------------------------- *)
+(* safe-spawns                                                               *)
+(* ------------------------------------------------------------------------- *)
+
+(* A term has safe spawns if all of its spawns have no mutable references. *)
+Inductive safe_spawns : tm -> Prop :=
+  | ss_unit :
+      safe_spawns <{unit}>
+
+  | ss_num : forall n,
+      safe_spawns <{N n}>
+
+  | ss_ref : forall ad T,
+      safe_spawns <{&ad :: T}>
+
+  | ss_new : forall T t,
+      safe_spawns t ->
+      safe_spawns <{new T t}>
+
+  | ss_load : forall t,
+      safe_spawns t ->
+      safe_spawns <{*t}>
+
+  | ss_asg : forall t1 t2,
+      safe_spawns t1 ->
+      safe_spawns t2 ->
+      safe_spawns <{t1 = t2}>
+
+  | ss_var : forall x,
+      safe_spawns <{var x}>
+
+  | ss_fun : forall x Tx t,
+      safe_spawns t ->
+      safe_spawns <{fn x Tx t}>
+
+  | ss_call : forall t1 t2,
+      safe_spawns t1 ->
+      safe_spawns t2 ->
+      safe_spawns <{call t1 t2}>
+
+  | ss_seq : forall t1 t2,
+      safe_spawns t1 ->
+      safe_spawns t2 ->
+      safe_spawns <{t1; t2}>
+
+  | ss_spawn : forall t,
+      no_mut t ->
+      safe_spawns <{spawn t}>
+  .
+
+(* ------------------------------------------------------------------------- *)
+(* has-var                                                                   *)
+(* ------------------------------------------------------------------------- *)
+
+Inductive has_var (x : id) : tm  -> Prop :=
+  | hv_new : forall T t,
+    has_var x t ->
+    has_var x <{new T t}>
+
+  | hv_load : forall t,
+    has_var x t ->
+    has_var x <{*t}>
+
+  | hv_asg1 : forall t1 t2,
+    has_var x t1 ->
+    has_var x <{t1 = t2}>
+
+  | hv_asg2 : forall t1 t2,
+    has_var x t2 ->
+    has_var x <{t1 = t2}>
+
+  | hv_var :
+    has_var x <{var x}>
+
+  | hv_fun : forall x' Tx t,
+    x <> x' ->
+    has_var x t ->
+    has_var x <{fn x' Tx t}>
+
+  | hv_call1 : forall t1 t2,
+    has_var x t1 ->
+    has_var x <{call t1 t2}>
+
+  | hv_call2 : forall t1 t2,
+    has_var x t2 ->
+    has_var x <{call t1 t2}>
+
+  | hv_seq1 : forall t1 t2,
+    has_var x t1 ->
+    has_var x <{t1; t2}>
+
+  | hv_seq2 : forall t1 t2,
+    has_var x t2 ->
+    has_var x <{t1; t2}>
+
+  | hv_spawn : forall t,
+    has_var x t ->
+    has_var x <{spawn t}>
+  .
+
+(* ------------------------------------------------------------------------- *)
+(* safe-memory-sharing                                                       *)
+(* ------------------------------------------------------------------------- *)
+
+Definition safe_memory_sharing m ths := forall tid1 tid2 ad,
+  tid1 <> tid2 ->
+  access ad m ths[tid2] ->
+  ~ unsafe_access ad m ths[tid1].
 
