SMS.v
@@ -1,9 +1,0 @@
-From Elo Require Import Core.
-From Elo Require Import Access.
-From Elo Require Import UnsafeAccess.
-
-Definition safe_memory_sharing m ths := forall tid1 tid2 ad,
-  tid1 <> tid2 ->
-  access ad m ths[tid2] ->
-  ~ unsafe_access ad m ths[tid1].
-
