Constructors.v
@@ -1,0 +1,140 @@
+From Elo Require Import Core.
+From Elo Require Import Definitions.
+From Elo Require Import Inversions.
+
+(* ------------------------------------------------------------------------- *)
+(* valid-addresses construction                                              *)
+(* ------------------------------------------------------------------------- *)
+
+Local Ltac solve_vad_construction := 
+  intros ** ? ?; inv_hasad; eauto.
+
+Local Lemma vad_unit : forall m,
+  valid_addresses m <{unit}>.
+Proof. solve_vad_construction. Qed.
+
+Local Lemma vad_num : forall m n,
+  valid_addresses m <{N n}>.
+Proof. solve_vad_construction. Qed.
+
+Local Lemma vad_ad : forall m ad T,
+  ad < #m ->
+  valid_addresses m <{&ad :: T}>.
+Proof. solve_vad_construction. Qed.
+
+Local Lemma vad_new : forall m t T,
+  valid_addresses m t ->
+  valid_addresses m <{new T t}>.
+Proof. solve_vad_construction. Qed.
+
+Local Lemma vad_load : forall m t,
+  valid_addresses m t ->
+  valid_addresses m <{*t}>.
+Proof. solve_vad_construction. Qed.
+
+Local Lemma vad_asg : forall m t1 t2,
+  valid_addresses m t1 ->
+  valid_addresses m t2 ->
+  valid_addresses m <{t1 = t2}>.
+Proof. solve_vad_construction. Qed.
+
+Local Lemma vad_var : forall m x,
+  valid_addresses m <{var x}>.
+Proof. solve_vad_construction. Qed.
+
+Local Lemma vad_fun : forall m x Tx t,
+  valid_addresses m t ->
+  valid_addresses m <{fn x Tx t}>.
+Proof. solve_vad_construction. Qed.
+
+Local Lemma vad_call : forall m t1 t2,
+  valid_addresses m t1 ->
+  valid_addresses m t2 ->
+  valid_addresses m <{call t1 t2}>.
+Proof. solve_vad_construction. Qed.
+
+Local Lemma vad_seq : forall m t1 t2,
+  valid_addresses m t1 ->
+  valid_addresses m t2 ->
+  valid_addresses m <{t1; t2}>.
+Proof. solve_vad_construction. Qed.
+
+Local Lemma vad_spawn : forall m t,
+  valid_addresses m t ->
+  valid_addresses m <{spawn t}>.
+Proof. solve_vad_construction. Qed.
+
+#[export] Hint Resolve
+  vad_unit vad_num
+  vad_ad vad_new vad_load vad_asg
+  vad_var vad_fun vad_call vad_seq vad_spawn
+  : vad.
+
+(* ------------------------------------------------------------------------- *)
+(* not-access constructors                                                   *)
+(* ------------------------------------------------------------------------- *)
+
+Local Ltac solve_nacc_construction :=
+  intros ** ?; invc_acc; contradiction.
+
+Lemma nacc_unit : forall m ad,
+  ~ access ad m <{unit}>.
+Proof.
+  intros ** ?. inv_acc.
+Qed.
+
+Lemma nacc_num : forall m ad n,
+  ~ access ad m <{N n}>.
+Proof. solve_nacc_construction. Qed.
+
+Lemma nacc_ref : forall m ad ad' T,
+  ad <> ad' ->
+  ~ access ad m m[ad'].tm ->
+  ~ access ad m <{&ad' :: T}>.
+Proof. solve_nacc_construction. Qed.
+
+Lemma nacc_new : forall m t ad T,
+  ~ access ad m t ->
+  ~ access ad m <{new T t}>.
+Proof. solve_nacc_construction. Qed.
+
+Lemma nacc_load : forall m t ad,
+  ~ access ad m t ->
+  ~ access ad m <{*t}>.
+Proof. solve_nacc_construction. Qed.
+
+Lemma nacc_asg : forall m t1 t2 ad,
+  ~ access ad m t1 ->
+  ~ access ad m t2 ->
+  ~ access ad m <{t1 = t2}>.
+Proof. solve_nacc_construction. Qed.
+
+Lemma nacc_fun : forall m x Tx t ad,
+  ~ access ad m t ->
+  ~ access ad m <{fn x Tx t}>.
+Proof. solve_nacc_construction. Qed.
+
+Lemma nacc_call : forall m t1 t2 ad,
+  ~ access ad m t1 ->
+  ~ access ad m t2 ->
+  ~ access ad m <{call t1 t2}>.
+Proof. solve_nacc_construction. Qed.
+
+Lemma nacc_seq : forall m t1 t2 ad,
+  ~ access ad m t1 ->
+  ~ access ad m t2 ->
+  ~ access ad m <{t1; t2}>.
+Proof. solve_nacc_construction. Qed.
+
+Lemma nacc_spawn : forall m t ad,
+  ~ access ad m <{spawn t}>.
+Proof. solve_nacc_construction. Qed.
+
+#[export] Hint Resolve
+  nacc_unit nacc_num
+  nacc_ref nacc_new nacc_load nacc_asg
+  nacc_fun nacc_call
+  nacc_seq
+  nacc_spawn
+  : acc.
+
