Inversions.v
@@ -1,0 +1,523 @@
+From Elo Require Import Core.
+From Elo Require Import Definitions.
+
+(* ------------------------------------------------------------------------- *)
+(* unfold hints                                                              *)
+(* ------------------------------------------------------------------------- *)
+
+#[export] Hint Unfold valid_addresses : vad.
+#[export] Hint Unfold well_typed_term : wtt.
+#[export] Hint Unfold valid_accesses  : vac.
+#[export] Hint Unfold safe_access     : sacc.
+
+#[export] Hint Extern 4 => unfold valid_addresses : vad.
+#[export] Hint Extern 4 => unfold well_typed_term : wtt.
+#[export] Hint Extern 4 => unfold valid_accesses  : vac.
+#[export] Hint Extern 4 => unfold safe_access     : sacc.
+
+(* ------------------------------------------------------------------------- *)
+(* has-address inversion                                                     *)
+(* ------------------------------------------------------------------------- *)
+
+Local Ltac match_hasad tactic :=
+  match goal with
+  | H : thread_default has_address _ |- _ => tactic H
+  | H : <{unit    }>   has_address _ |- _ => tactic H
+  | H : <{N _     }>   has_address _ |- _ => tactic H
+  | H : <{& _ :: _}>   has_address _ |- _ => tactic H
+  | H : <{new _ _ }>   has_address _ |- _ => tactic H
+  | H : <{* _     }>   has_address _ |- _ => tactic H
+  | H : <{_ = _   }>   has_address _ |- _ => tactic H
+  | H : <{var _   }>   has_address _ |- _ => tactic H
+  | H : <{fn _ _ _}>   has_address _ |- _ => tactic H
+  | H : <{call _ _}>   has_address _ |- _ => tactic H
+  | H : <{_ ; _   }>   has_address _ |- _ => tactic H
+  | H : <{spawn _ }>   has_address _ |- _ => tactic H
+  end.
+
+Ltac inv_hasad  := match_hasad inv.
+Ltac invc_hasad := match_hasad invc.
+
+(* ------------------------------------------------------------------------- *)
+(* valid-addresses inversion                                                 *)
+(* ------------------------------------------------------------------------- *)
+
+Local Ltac solve_vad_inversion := 
+  intros; try split; eauto using has_ad with vad.
+
+Local Lemma inv_vad_ref : forall m ad T,
+  valid_addresses m <{&ad :: T}> ->
+  ad < #m.
+Proof. solve_vad_inversion. Qed.
+
+Local Lemma inv_vad_new : forall m t T,
+  valid_addresses m <{new T t}> ->
+  valid_addresses m t.
+Proof. solve_vad_inversion. Qed.
+
+Local Lemma inv_vad_load : forall m t,
+  valid_addresses m <{*t}> ->
+  valid_addresses m t.
+Proof. solve_vad_inversion. Qed.
+
+Local Lemma inv_vad_asg : forall m t1 t2,
+  valid_addresses m <{t1 = t2}> ->
+  valid_addresses m t1 /\ valid_addresses m t2.
+Proof. solve_vad_inversion. Qed.
+
+Local Lemma inv_vad_fun : forall m x Tx t,
+  valid_addresses m <{fn x Tx t}> ->
+  valid_addresses m t.
+Proof. solve_vad_inversion. Qed.
+
+Local Lemma inv_vad_call : forall m t1 t2,
+  valid_addresses m <{call t1 t2}> ->
+  valid_addresses m t1 /\ valid_addresses m t2.
+Proof. solve_vad_inversion. Qed.
+
+Local Lemma inv_vad_seq : forall m t1 t2,
+  valid_addresses m <{t1; t2}> ->
+  valid_addresses m t1 /\ valid_addresses m t2.
+Proof. solve_vad_inversion. Qed.
+
+Local Lemma inv_vad_spawn : forall m t,
+  valid_addresses m <{spawn t}> ->
+  valid_addresses m t.
+Proof. solve_vad_inversion. Qed.
+
+Ltac inv_vad :=
+ match goal with
+ (* irrelevant for unit *)
+ (* irrelevant for num  *)
+ | H : valid_addresses _ <{& _ :: _}> |- _ => eapply inv_vad_ref   in H as ?
+ | H : valid_addresses _ <{new _ _ }> |- _ => eapply inv_vad_new   in H
+ | H : valid_addresses _ <{* _     }> |- _ => eapply inv_vad_load  in H
+ | H : valid_addresses _ <{_ = _   }> |- _ => eapply inv_vad_asg   in H as [? ?]
+ (* irrelevant for var  *)
+ | H : valid_addresses _ <{fn _ _ _}> |- _ => eapply inv_vad_fun   in H
+ | H : valid_addresses _ <{call _ _}> |- _ => eapply inv_vad_call  in H as [? ?]
+ | H : valid_addresses _ <{_ ; _   }> |- _ => eapply inv_vad_seq   in H as [? ?]
+ | H : valid_addresses _ <{spawn _ }> |- _ => eapply inv_vad_spawn in H
+ end.
+
+(* ------------------------------------------------------------------------- *)
+(* well-typed-term inversion                                                 *)
+(* ------------------------------------------------------------------------- *)
+
+Local Ltac solve_wtt_inversion := 
+  intros * [? ?]; try split; inv_type; try discriminate; eauto; eexists; eauto.
+
+Local Lemma inv_wtt_ref : forall ad T,
+  well_typed_term <{&ad :: T}> ->
+  (exists T', T = <{{&T'}}>) \/ (exists T', T = <{{i&T'}}>).
+Proof. solve_wtt_inversion. Qed.
+
+Local Lemma inv_wtt_new : forall t T,
+  well_typed_term <{new T t}> ->
+  well_typed_term t.
+Proof. solve_wtt_inversion. Qed.
+
+Local Lemma inv_wtt_load : forall t,
+  well_typed_term <{*t}> ->
+  well_typed_term t.
+Proof. solve_wtt_inversion. Qed.
+
+Local Lemma inv_wtt_asg : forall t1 t2,
+  well_typed_term <{t1 = t2}> ->
+  well_typed_term t1 /\ well_typed_term t2.
+Proof. solve_wtt_inversion. Qed.
+
+Local Lemma inv_wtt_var : forall x,
+  well_typed_term <{var x}> ->
+  False.
+Proof. solve_wtt_inversion. Qed.
+
+Local Lemma inv_wtt_fun : forall x Tx t,
+  well_typed_term <{fn x Tx t}> ->
+  exists T, empty[x <== Tx] |-- t is T.
+Proof. solve_wtt_inversion. Qed.
+
+Local Lemma inv_wtt_call : forall t1 t2,
+  well_typed_term <{call t1 t2}> ->
+  well_typed_term t1 /\ well_typed_term t2.
+Proof. solve_wtt_inversion. Qed.
+
+Local Lemma inv_wtt_seq : forall t1 t2,
+  well_typed_term <{t1; t2}> ->
+  well_typed_term t1 /\ well_typed_term t2.
+Proof. solve_wtt_inversion. Qed.
+
+Local Lemma inv_wtt_spawn : forall t,
+  well_typed_term <{spawn t}> ->
+  well_typed_term t.
+Proof. solve_wtt_inversion. Qed.
+
+Ltac inv_wtt :=
+  match goal with
+  (* irrelevant for unit *)
+  (* irrelevant for num  *)
+  | H : well_typed_term <{& _ :: _}> |- _ =>
+      eapply inv_wtt_ref   in H as [[? ?] | [? ?]]
+  | H : well_typed_term <{new _ _ }> |- _ =>
+      eapply inv_wtt_new   in H
+  | H : well_typed_term <{* _     }> |- _ =>
+      eapply inv_wtt_load  in H
+  | H : well_typed_term <{_ = _   }> |- _ =>
+      eapply inv_wtt_asg   in H as [? ?]
+  | H : well_typed_term <{fn _ _ _}> |- _ =>
+      eapply inv_wtt_fun   in H as [? ?]
+  | H : well_typed_term <{call _ _}> |- _ =>
+      eapply inv_wtt_call  in H as [? ?]
+  | H : well_typed_term <{_ ; _   }> |- _ =>
+      eapply inv_wtt_seq   in H as [? ?]
+  | H : well_typed_term <{spawn _ }> |- _ =>
+      eapply inv_wtt_spawn in H
+  end.
+
+(* ------------------------------------------------------------------------- *)
+(* consistently-typed-references inversion                                   *)
+(* ------------------------------------------------------------------------- *)
+
+Local Ltac match_ctr tactic :=
+  match goal with
+  (* irrelevant for unit *)
+  (* irrelevant for num  *)
+  | H : consistently_typed_references _ <{& _ :: _}> |- _ => tactic H
+  | H : consistently_typed_references _ <{new _ _ }> |- _ => tactic H
+  | H : consistently_typed_references _ <{* _     }> |- _ => tactic H
+  | H : consistently_typed_references _ <{_ = _   }> |- _ => tactic H
+  (* irrelevant for var  *)
+  | H : consistently_typed_references _ <{fn _ _ _}> |- _ => tactic H
+  | H : consistently_typed_references _ <{call _ _}> |- _ => tactic H
+  | H : consistently_typed_references _ <{_ ; _   }> |- _ => tactic H
+  | H : consistently_typed_references _ <{spawn _ }> |- _ => tactic H
+  end.
+
+Ltac inv_ctr  := match_ctr inv.
+Ltac invc_ctr := match_ctr invc.
+
+(* ------------------------------------------------------------------------- *)
+(* access inversion                                                          *)
+(* ------------------------------------------------------------------------- *)
+
+Local Ltac match_acc tactic :=
+  match goal with
+  | H : access _ _ thread_default |- _ => tactic H
+  | H : access _ _ <{unit    }>   |- _ => tactic H
+  | H : access _ _ <{N _     }>   |- _ => tactic H
+  | H : access _ _ <{& _ :: _}>   |- _ => tactic H
+  | H : access _ _ <{new _ _ }>   |- _ => tactic H
+  | H : access _ _ <{* _     }>   |- _ => tactic H
+  | H : access _ _ <{_ = _   }>   |- _ => tactic H
+  | H : access _ _ <{var _   }>   |- _ => tactic H
+  | H : access _ _ <{fn _ _ _}>   |- _ => tactic H
+  | H : access _ _ <{call _ _}>   |- _ => tactic H
+  | H : access _ _ <{_ ; _   }>   |- _ => tactic H
+  | H : access _ _ <{spawn _ }>   |- _ => tactic H
+  end.
+
+Ltac inv_acc  := match_acc inv.
+Ltac invc_acc := match_acc invc.
+
+(* ------------------------------------------------------------------------- *)
+(* valid-accesses inversion                                                  *)
+(* ------------------------------------------------------------------------- *)
+
+Local Ltac solve_vac_inversion := 
+  intros; autounfold with vac in *; try split; eauto using access.
+
+Local Lemma inv_vac_ref : forall m ad T,
+  valid_accesses m <{&ad :: T}> ->
+  ad < #m /\ valid_accesses m m[ad].tm.
+Proof.
+  solve_vac_inversion. intros ad'.
+  destruct (nat_eq_dec ad ad'); subst; eauto using access.
+Qed.
+
+Local Lemma inv_vac_new : forall m t T,
+  valid_accesses m <{new T t}> ->
+  valid_accesses m t.
+Proof. solve_vac_inversion. Qed.
+
+Local Lemma inv_vac_load : forall m t,
+  valid_accesses m <{*t}> ->
+  valid_accesses m t.
+Proof. solve_vac_inversion. Qed.
+
+Local Lemma inv_vac_asg : forall m t1 t2,
+  valid_accesses m <{t1 = t2}> ->
+  valid_accesses m t1 /\ valid_accesses m t2.
+Proof. solve_vac_inversion. Qed.
+
+Local Lemma inv_vac_fun : forall m x Tx t,
+  valid_accesses m <{fn x Tx t}> ->
+  valid_accesses m t.
+Proof. solve_vac_inversion. Qed.
+
+Local Lemma inv_vac_call : forall m t1 t2,
+  valid_accesses m <{call t1 t2}> ->
+  valid_accesses m t1 /\ valid_accesses m t2.
+Proof. solve_vac_inversion. Qed.
+
+Local Lemma inv_vac_seq : forall m t1 t2,
+  valid_accesses m <{t1; t2}> ->
+  valid_accesses m t1 /\ valid_accesses m t2.
+Proof. solve_vac_inversion. Qed.
+
+Ltac inv_vac :=
+  match goal with
+  (* irrelevant for unit  *)
+  (* irrelevant for num   *)
+  | H : valid_accesses _ <{& _ :: _}> |- _ => eapply inv_vac_ref  in H as [? ?]
+  | H : valid_accesses _ <{new _ _ }> |- _ => eapply inv_vac_new  in H
+  | H : valid_accesses _ <{* _     }> |- _ => eapply inv_vac_load in H
+  | H : valid_accesses _ <{_ = _   }> |- _ => eapply inv_vac_asg  in H as [? ?]
+  (* irrelevant for var   *)                    
+  | H : valid_accesses _ <{fn _ _ _}> |- _ => eapply inv_vac_fun  in H
+  | H : valid_accesses _ <{call _ _}> |- _ => eapply inv_vac_call in H as [? ?]
+  | H : valid_accesses _ <{_ ; _   }> |- _ => eapply inv_vac_seq  in H as [? ?]
+  (* irrelevant for spawn *)                    
+  end.
+
+(* ------------------------------------------------------------------------- *)
+(* not-access inversion                                                      *)
+(* ------------------------------------------------------------------------- *)
+
+Local Ltac solve_nacc_inversion := 
+  intros; try split; eauto using access.
+
+Local Lemma inv_nacc_ref : forall m ad ad' T,
+  ~ access ad m <{&ad' :: T}> ->
+  ad <> ad' /\ ~ access ad m (m[ad'].tm).
+Proof.
+  intros. assert (ad <> ad') by (intros ?; subst; eauto using access).
+  split; eauto using access.
+Qed.
+
+Local Lemma inv_nacc_new : forall m t ad T,
+  ~ access ad m <{new T t}> ->
+  ~ access ad m t.
+Proof. solve_nacc_inversion. Qed.
+
+Local Lemma inv_nacc_load : forall m t ad,
+  ~ access ad m <{*t}> ->
+  ~ access ad m t.
+Proof. solve_nacc_inversion. Qed.
+
+Local Lemma inv_nacc_asg : forall m t1 t2 ad,
+  ~ access ad m <{t1 = t2}> ->
+  ~ access ad m t1 /\ ~ access ad m t2.
+Proof. solve_nacc_inversion. Qed.
+
+Local Lemma inv_nacc_fun : forall m x Tx t ad,
+  ~ access ad m <{fn x Tx t}> ->
+  ~ access ad m t.
+Proof. solve_nacc_inversion. Qed.
+
+Local Lemma inv_nacc_call : forall m t1 t2 ad,
+  ~ access ad m <{call t1 t2}> ->
+  ~ access ad m t1 /\ ~ access ad m t2.
+Proof. solve_nacc_inversion. Qed.
+
+Local Lemma inv_nacc_seq : forall m t1 t2 ad,
+  ~ access ad m <{t1; t2}> ->
+  ~ access ad m t1 /\ ~ access ad m t2.
+Proof. solve_nacc_inversion. Qed.
+
+Ltac inv_nacc :=
+  match goal with
+  (* irrelevant for unit  *)
+  (* irrelevant for num   *)
+  | H : ~ access _ _ <{& _ :: _}> |- _ => eapply inv_nacc_ref   in H as [? ?]
+  | H : ~ access _ _ <{new _ _ }> |- _ => eapply inv_nacc_new  in H
+  | H : ~ access _ _ <{* _     }> |- _ => eapply inv_nacc_load in H
+  | H : ~ access _ _ <{_ = _   }> |- _ => eapply inv_nacc_asg  in H as [? ?]
+  (* irrelevant for var   *)                    
+  | H : ~ access _ _ <{fn _ _ _}> |- _ => eapply inv_nacc_fun  in H
+  | H : ~ access _ _ <{call _ _}> |- _ => eapply inv_nacc_call in H as [? ?]
+  | H : ~ access _ _ <{_ ; _   }> |- _ => eapply inv_nacc_seq  in H as [? ?]
+  (* irrelevant for spawn *)                    
+  end.
+
+(* ------------------------------------------------------------------------- *)
+(* unsafe-access inversion                                                   *)
+(* ------------------------------------------------------------------------- *)
+
+Local Ltac match_uacc tactic :=
+  match goal with
+  | H : unsafe_access _ _ thread_default |- _ => tactic H
+  | H : unsafe_access _ _ <{unit    }>   |- _ => tactic H
+  | H : unsafe_access _ _ <{N _     }>   |- _ => tactic H
+  | H : unsafe_access _ _ <{& _ :: _}>   |- _ => tactic H
+  | H : unsafe_access _ _ <{new _ _ }>   |- _ => tactic H
+  | H : unsafe_access _ _ <{* _     }>   |- _ => tactic H
+  | H : unsafe_access _ _ <{_ = _   }>   |- _ => tactic H
+  | H : unsafe_access _ _ <{var _   }>   |- _ => tactic H
+  | H : unsafe_access _ _ <{fn _ _ _}>   |- _ => tactic H
+  | H : unsafe_access _ _ <{call _ _}>   |- _ => tactic H
+  | H : unsafe_access _ _ <{_ ; _   }>   |- _ => tactic H
+  | H : unsafe_access _ _ <{spawn _ }>   |- _ => tactic H
+  end.
+
+Ltac inv_uacc  := match_uacc inv.
+Ltac invc_uacc := match_uacc invc.
+
+(* ------------------------------------------------------------------------- *)
+(* not-unsafe-access inversion                                               *)
+(* ------------------------------------------------------------------------- *)
+
+Local Lemma inv_nuacc_ref_eq : forall m ad T,
+  ~ unsafe_access ad m <{&ad :: &T}> ->
+  False.
+Proof. eauto using unsafe_access. Qed.
+
+Local Lemma inv_nuacc_ref_neqM : forall m ad ad' T,
+  ~ unsafe_access ad m <{&ad' :: &T}> ->
+  (ad <> ad' /\ ~ unsafe_access ad m m[ad'].tm).
+Proof.
+  intros. destruct (nat_eq_dec ad ad'); subst; eauto using unsafe_access.
+  exfalso. eauto using inv_nuacc_ref_eq.
+Qed.
+
+Lemma inv_nuacc_ref_neqI : forall m ad ad' T,
+  forall_memory m value ->
+  consistently_typed_references m <{&ad' :: i&T}> ->
+  (* --- *)
+  ~ unsafe_access ad m <{&ad' :: i&T}> ->
+  ~ unsafe_access ad m m[ad'].tm.
+Proof.
+  intros * Hval **. invc_ctr. intros ?.
+  specialize (Hval ad'); simpl in *.
+  destruct Hval; inv_type; inv_uacc; eauto.
+Qed.
+
+Local Ltac solve_nuacc_inversion :=
+  intros; try (split; intros); eauto using unsafe_access.
+
+Local Lemma inv_nuacc_new : forall m t ad T,
+  ~ unsafe_access ad m <{new T t}> ->
+  ~ unsafe_access ad m t.
+Proof. solve_nuacc_inversion. Qed.
+
+Local Lemma inv_nuacc_load : forall m t ad,
+  ~ unsafe_access ad m <{*t}> ->
+  ~ unsafe_access ad m t.
+Proof. solve_nuacc_inversion. Qed.
+
+Local Lemma inv_nuacc_asg : forall m t1 t2 ad,
+  ~ unsafe_access ad m <{t1 = t2}> ->
+  ~ unsafe_access ad m t1 /\ ~ unsafe_access ad m t2.
+Proof. solve_nuacc_inversion. Qed.
+
+Local Lemma inv_nuacc_fun : forall m t ad x Tx,
+  ~ unsafe_access ad m <{fn x Tx t}> ->
+  ~ unsafe_access ad m t.
+Proof. solve_nuacc_inversion. Qed.
+
+Local Lemma inv_nuacc_call : forall m t1 t2 ad,
+  ~ unsafe_access ad m <{call t1 t2}> ->
+  ~ unsafe_access ad m t1 /\ ~ unsafe_access ad m t2.
+Proof. solve_nuacc_inversion. Qed.
+
+Local Lemma inv_nuacc_seq : forall m t1 t2 ad,
+  ~ unsafe_access ad m <{t1; t2}> ->
+  ~ unsafe_access ad m t1 /\ ~ unsafe_access ad m t2.
+Proof. solve_nuacc_inversion. Qed.
+
+Ltac inv_nuacc :=
+  match goal with
+  | H : ~ unsafe_access ?ad _ <{& ?ad  :: & _ }> |- _ =>
+    eapply inv_nuacc_ref_eq   in H; solve contradiction
+  | H : ~ unsafe_access ?ad _ <{& ?ad' :: & _ }> |- _ =>
+    eapply inv_nuacc_ref_neqM in H as [? ?]
+  | H : ~ unsafe_access _ _   <{new _ _       }> |- _ =>
+    eapply inv_nuacc_new     in H
+  | H : ~ unsafe_access _ _   <{* _           }> |- _ =>
+    eapply inv_nuacc_load    in H
+  | H : ~ unsafe_access _ _   <{_ = _         }> |- _ =>
+    eapply inv_nuacc_asg     in H as [? ?]
+  | H : ~ unsafe_access _ _   <{fn _ _ _      }> |- _ =>
+    eapply inv_nuacc_fun     in H
+  | H : ~ unsafe_access _ _   <{call _ _      }> |- _ =>
+    eapply inv_nuacc_call    in H as [? ?]
+  | H : ~ unsafe_access _ _   <{_ ; _         }> |- _ =>
+    eapply inv_nuacc_seq     in H as [? ?]
+
+  | Hval   : forall_memory ?m value,
+    Hctr   : consistently_typed_references ?m <{& ?ad' :: (i& ?T) }>,
+    Hnuacc : ~ unsafe_access ?ad ?m <{& ?ad' :: (i& ?T) }> |- _ =>
+    eapply (inv_nuacc_ref_neqI m ad ad' T Hval Hctr) in Hnuacc
+  end.
+
+(* ------------------------------------------------------------------------- *)
+(* no-mut inversion                                                          *)
+(* ------------------------------------------------------------------------- *)
+
+Local Ltac match_nomut tactic :=
+  match goal with
+  (* irrelevant for unit      *)
+  (* irrelevant for num       *)
+  | H : no_mut <{& _ :: Unit     }> |- _ => tactic H
+  | H : no_mut <{& _ :: Num      }> |- _ => tactic H
+  (* irrelevant if &ad :: i&T *)
+  | H : no_mut <{& _ :: & _      }> |- _ => tactic H
+  | H : no_mut <{& _ :: (_ --> _)}> |- _ => tactic H
+  | H : no_mut <{new _ _         }> |- _ => tactic H
+  | H : no_mut <{* _             }> |- _ => tactic H
+  | H : no_mut <{_ = _           }> |- _ => tactic H
+  (* irrelevant for var       *)
+  | H : no_mut <{fn _ _ _        }> |- _ => tactic H
+  | H : no_mut <{call _ _        }> |- _ => tactic H
+  | H : no_mut <{_ ; _           }> |- _ => tactic H
+  | H : no_mut <{spawn _         }> |- _ => tactic H
+  end.
+
+Ltac inv_nomut  := match_nomut inv.
+Ltac invc_nomut := match_nomut invc.
+
+(* ------------------------------------------------------------------------- *)
+(* safe-spawns inversion                                                     *)
+(* ------------------------------------------------------------------------- *)
+
+Local Ltac match_ss tactic :=
+  match goal with
+  (* irrelevant for unit *)
+  (* irrelevant for num  *)
+  (* irrelevant for ad   *)
+  | H : safe_spawns <{new _ _ }> |- _ => tactic H
+  | H : safe_spawns <{* _     }> |- _ => tactic H
+  | H : safe_spawns <{_ = _   }> |- _ => tactic H
+  (* irrelevant for var  *)
+  | H : safe_spawns <{fn _ _ _}> |- _ => tactic H
+  | H : safe_spawns <{call _ _}> |- _ => tactic H
+  | H : safe_spawns <{_ ; _   }> |- _ => tactic H
+  | H : safe_spawns <{spawn _ }> |- _ => tactic H
+  end.
+
+Ltac inv_ss  := match_ss inv.
+Ltac invc_ss := match_ss invc.
+
+(* ------------------------------------------------------------------------- *)
+(* has-var inversion                                                         *)
+(* ------------------------------------------------------------------------- *)
+
+Local Ltac match_hasvar tactic :=
+  match goal with
+  | H : has_var _  thread_default |- _ => tactic H
+  | H : has_var _  <{unit    }>   |- _ => tactic H
+  | H : has_var _  <{N _     }>   |- _ => tactic H
+  | H : has_var _  <{& _ :: _}>   |- _ => tactic H
+  | H : has_var _  <{new _ _ }>   |- _ => tactic H
+  | H : has_var _  <{* _     }>   |- _ => tactic H
+  | H : has_var _  <{_ = _   }>   |- _ => tactic H
+  | H : has_var ?x <{var ?x  }>   |- _ => fail
+  | H : has_var ?x <{var ?y  }>   |- _ => tactic H
+  | H : has_var _  <{fn _ _ _}>   |- _ => tactic H
+  | H : has_var _  <{call _ _}>   |- _ => tactic H
+  | H : has_var _  <{_ ; _   }>   |- _ => tactic H
+  | H : has_var _  <{spawn _ }>   |- _ => tactic H
+  end.
+
+Ltac inv_hasvar  := match_hasvar inv.
+Ltac invc_hasvar := match_hasvar invc.
+
