Lemmas.v
@@ -1,0 +1,37 @@
+From Elo Require Import Core.
+From Elo Require Import Properties.
+
+Lemma consistently_typed_write_effect : forall m t t' ad v T,
+  valid_addresses m t ->
+  well_typed_term t ->
+  consistently_typed_references m t ->
+  (* --- *)
+  t --[EF_Write ad v T]--> t' ->
+  exists Tv, T = <{{&Tv}}>
+          /\ empty |-- v is Tv
+          /\ empty |-- m[ad].tm is Tv
+          /\ m[ad].typ = <{{&Tv}}>.
+Proof.
+  intros * ? Hwtt **. inversion Hwtt as [T' ?].
+  clear Hwtt. generalize dependent T'.
+  induction_tstep; intros; inv_vad; inv_type; inv_ctr; eauto.
+  inv_type. inv_ctr. eauto.
+Qed.
+
+Lemma nacc_vad_length : forall m t,
+  forall_memory m (valid_addresses m) ->
+  valid_addresses m t ->
+  ~ access (#m) m t.
+Proof.
+  intros * ? Hvad Hacc. remember (#m) as ad.
+  induction Hacc; inv_vad; eauto. rewrite Heqad in *. eauto.
+Qed.
+
+Corollary nuacc_vad_length : forall m t,
+  forall_memory m (valid_addresses m) ->
+  valid_addresses m t ->
+  ~ unsafe_access (#m) m t.
+Proof.
+  eauto using nacc_then_nuacc, nacc_vad_length.
+Qed.
+
