Sanity.v
@@ -1,6 +1,0 @@
-From Elo Require Import Util.
-From Elo Require Import Core.
-
-From Elo Require Import Definitions.
-
-(* TODO: has-address *)
