Sem.v
@@ -1,0 +1,369 @@
+From Coq Require Import Arith.
+From Coq Require Import Strings.String.
+From Coq Require Import List.
+From Coq Require Import Lia.
+
+From Elo Require Import Util.
+From Elo Require Import Array.
+From Elo Require Import Map.
+ 
+(* ------------------------------------------------------------------------- *)
+(* types                                                                     *)
+(* ------------------------------------------------------------------------- *)
+
+(* immutable type *)
+Inductive ityp : Set :=
+  | TY_Unit
+  | TY_Num
+  | TY_RefI : ityp -> ityp
+  .
+
+(* type *)
+Inductive typ : Set :=
+  | TY_Immut : ityp -> typ
+  | TY_RefM  : typ  -> typ
+  | TY_Fun   : typ  -> typ -> typ
+  .
+
+(* ------------------------------------------------------------------------- *)
+(* terms                                                                     *)
+(* ------------------------------------------------------------------------- *)
+
+Definition id := string.
+Definition num := nat.
+
+Inductive tm : Set :=
+  (* primitives *)
+  | TM_Unit
+  | TM_Num   : num -> tm
+  (* memory *)
+  | TM_Ref   : num -> typ -> tm
+  | TM_New   : typ -> tm  -> tm
+  | TM_Load  : tm  -> tm
+  | TM_Asg   : tm  -> tm  -> tm
+  (* functions *)
+  | TM_Var   : id  -> tm
+  | TM_Fun   : id  -> typ -> tm -> tm
+  | TM_Call  : tm  -> tm  -> tm
+  (* sequencing *)
+  | TM_Seq   : tm  -> tm  -> tm
+  (* concurrency *)
+  | TM_Spawn : tm  -> tm
+  .
+
+(* ------------------------------------------------------------------------- *)
+(* notations                                                                 *)
+(* ------------------------------------------------------------------------- *)
+
+Declare Custom Entry elo_typ.
+Notation "<{{ T }}>" := T (T custom elo_typ at level 99).
+Notation "( x )"     := x (in custom elo_typ, x at level 99).
+Notation "x"         := x (in custom elo_typ at level 0, x constr at level 0).
+
+Notation "'Unit'"      := (TY_Immut TY_Unit)     (in custom elo_typ at level 0).
+Notation "'Num'"       := (TY_Immut TY_Num)      (in custom elo_typ at level 0).
+Notation "'Immut' T"   := (TY_Immut T)           (in custom elo_typ at level 5).
+Notation "'&' T"       := (TY_RefM T)            (in custom elo_typ at level 5).
+Notation "'i&' T"      := (TY_Immut (TY_RefI T)) (in custom elo_typ at level 5).
+Notation "T1 '-->' T2" := (TY_Fun T1 T2)         (in custom elo_typ at level 50,
+                                                           right associativity).
+
+Declare Custom Entry elo_tm.
+Notation "<{ t }>" := t (t custom elo_tm at level 99).
+Notation "x"       := x (in custom elo_tm at level 0, x constr at level 0).
+
+Notation "'unit'"        := (TM_Unit)       (in custom elo_tm at level 0).
+Notation "'N' n"         := (TM_Num n)      (in custom elo_tm at level 0).
+Notation "'&' ad '::' T" := (TM_Ref ad T)    (in custom elo_tm at level 0,
+                                             T custom elo_typ at level 0).
+Notation "'new' T t"     := (TM_New T t)     (in custom elo_tm at level 0,
+                                             T custom elo_typ at level 0).
+Notation "'*' t"         := (TM_Load t)     (in custom elo_tm at level 0).
+Notation "t1 '=' t2"     := (TM_Asg t1 t2)  (in custom elo_tm at level 70,
+                                                        no associativity).
+Notation "'var' x"       := (TM_Var x)      (in custom elo_tm at level 0).
+Notation "'fn' x Tx t"   := (TM_Fun x Tx t)  (in custom elo_tm at level 0,
+                                                      x constr at level 0,
+                                            Tx custom elo_typ at level 0).
+Notation "'call' t1 t2"  := (TM_Call t1 t2) (in custom elo_tm at level 0).
+Notation "t1 ';' t2"     := (TM_Seq t1 t2)   (in custom elo_tm at level 2,
+                                                     right associativity).
+Notation "'spawn' t"     := (TM_Spawn t)    (in custom elo_tm at level 0).
+
+Reserved Notation "'[' x ':=' tx ']' t"
+  (at level 20, x constr, tx at next level, t at next level).
+Reserved Notation "t '--[' e ']-->' t'"
+  (at level 40, e at next level, t' at next level).
+Reserved Notation "m / t '==[' e ']==>' m' / t'"
+  (at level 40, t at next level, e at next level, m' at next level).
+Reserved Notation "m / ths '~~[' tid , e ']~~>' m' / ths'"
+  (at level 40, ths at next level, tid at next level, e at next level,
+                m' at next level).
+Reserved Notation "m / t '~~[' tc ']~~>*' m' / t'"
+  (at level 40, t at next level, tc at next level,
+                m' at next level, t' at next level).
+Reserved Notation "Gamma '|--' t 'is' T"
+  (at level 40).
+
+(* ------------------------------------------------------------------------- *)
+(* values                                                                    *)
+(* ------------------------------------------------------------------------- *)
+
+Inductive value : tm -> Prop :=
+  | V_Unit : value <{ unit }> 
+  | V_Num : forall n, value <{ N n }>
+  | V_Ref : forall ad T, value <{ &ad :: T }>
+  | V_Fun : forall x Tx t, value <{ fn x Tx t }>
+  .
+
+(* ------------------------------------------------------------------------- *)
+(* effects                                                                   *)
+(* ------------------------------------------------------------------------- *)
+
+Definition addr := nat.
+
+Inductive eff : Set :=
+  | EF_None
+  | EF_Alloc (ad : addr) (v : tm) (T : typ)
+  | EF_Read  (ad : addr) (v : tm)
+  | EF_Write (ad : addr) (v : tm) (T : typ)
+  | EF_Spawn (t : tm)
+  .
+
+(* ------------------------------------------------------------------------- *)
+(* typing                                                                    *)
+(* ------------------------------------------------------------------------- *)
+
+Definition ctx := map typ.
+
+(* Filters out of the context all variables with non-immutable types. *)
+Definition safe (Gamma : ctx) : ctx :=
+  fun k => 
+    match Gamma k with
+    | Some <{{ Immut T }}> => Some <{{ Immut T }}>
+    | _ => None
+    end.
+
+Inductive type_of : ctx -> tm -> typ -> Prop :=
+  | T_Unit : forall Gamma,
+    Gamma |-- <{ unit }> is <{{ Unit }}>
+
+  | T_Num : forall Gamma n,
+    Gamma |-- <{ N n }> is <{{ Num }}>
+
+  | T_RefM : forall Gamma ad T,
+    Gamma |-- <{ &ad :: &T }> is <{{ &T }}>
+
+  | T_RefI : forall Gamma ad T,
+    Gamma |-- <{ &ad :: i&T }> is <{{ i&T }}>
+
+  | T_NewM : forall Gamma t T,
+    Gamma |-- t is T ->
+    Gamma |-- <{ new &T t }> is <{{ &T }}>
+
+  | T_NewI : forall Gamma t T,
+    Gamma |-- t is <{{ Immut T }}> ->
+    Gamma |-- <{ new i&T t }> is <{{ i&T }}>
+
+  | T_LoadM : forall Gamma t T,
+    Gamma |-- t is <{{ &T }}> ->
+    Gamma |-- <{ *t }> is T
+
+  | T_LoadI : forall Gamma t T,
+    Gamma |-- t is <{{ i&T }}> ->
+    Gamma |-- <{ *t }> is <{{ Immut T }}>
+
+  | T_Asg : forall Gamma t1 t2 T,
+    Gamma |-- t1 is <{{ &T }}> ->
+    Gamma |-- t2 is T ->
+    Gamma |-- <{ t1 = t2 }> is <{{ Unit }}>
+
+  | T_Var : forall Gamma x T,
+    Gamma x = Some T ->
+    Gamma |-- <{ var x }> is T
+
+  | T_Fun : forall Gamma x t T Tx,
+    Gamma[x <== Tx] |-- t is T ->
+    Gamma |-- <{ fn x Tx t }> is <{{ Tx --> T }}>
+
+  | T_Call : forall Gamma t1 t2 Tx T,
+    Gamma |-- t1 is <{{ Tx --> T }}> ->
+    Gamma |-- t2 is Tx ->
+    Gamma |-- <{ call t1 t2 }> is T
+
+  | T_Seq : forall Gamma t1 t2 T1 T2,
+    Gamma |-- t1 is T1 ->
+    Gamma |-- t2 is T2 ->
+    Gamma |-- <{ t1; t2 }> is T2
+
+  | T_Spawn : forall Gamma t T,
+    safe Gamma |-- t is T ->
+    Gamma |-- <{ spawn t }> is <{{ Unit }}> 
+
+  where "Gamma '|--' t 'is' T" := (type_of Gamma t T).
+
+(* ------------------------------------------------------------------------- *)
+(* substitution                                                              *)
+(* ------------------------------------------------------------------------- *)
+
+Local Infix "=?" := string_dec (at level 70, no associativity).
+
+Fixpoint subst (x : id) (tx t : tm) : tm :=
+  match t with
+  | <{ unit        }> => t
+  | <{ N _         }> => t
+  | <{ & _ :: _    }> => t
+  | <{ new T t'    }> => <{ new T ([x := tx] t')            }>
+  | <{ *t'         }> => <{ * ([x := tx] t')                }>
+  | <{ t1 = t2     }> => <{ ([x := tx] t1) = ([x := tx] t2) }>
+  | <{ var x'      }> => if x =? x' then tx else t
+  | <{ fn x' Tx t' }> => if x =? x' then t  else <{ fn x' Tx ([x := tx] t') }>
+  | <{ call t1 t2  }> => <{ call ([x := tx] t1) ([x := tx] t2) }>
+  | <{ t1; t2      }> => <{ ([x := tx] t1) ; ([x := tx] t2)    }>
+  | <{ spawn t'    }> => <{ spawn ([x := tx] t')               }>
+  end
+  where "'[' x ':=' tx ']' t" := (subst x tx t).
+
+(* ------------------------------------------------------------------------- *)
+(* operational semantics -- term step                                        *)
+(* ------------------------------------------------------------------------- *)
+
+Inductive tstep : tm -> eff -> tm -> Prop :=
+  (* New *)
+  | TS_New1 : forall t t' e T,
+    t --[e]--> t' ->
+    <{ new T t }> --[e]--> <{ new T t' }>
+
+  | TS_New : forall ad v T,
+    value v ->
+    <{ new T v }> --[EF_Alloc ad v T]--> <{ &ad :: T }>
+
+  (* Load *)
+  | TS_Load1 : forall t t' e,
+    t --[e]--> t' ->
+    <{ *t }> --[e]--> <{ *t' }>
+
+  | TS_Load : forall ad t T,
+    <{ * &ad :: T }> --[EF_Read ad t]--> t
+
+  (* Asg *)
+  | TS_Asg1 : forall t1 t1' t2 e,
+    t1 --[e]--> t1' ->
+    <{ t1 = t2 }> --[e]--> <{ t1' = t2 }>
+
+  | TS_Asg2 : forall t t' v e,
+    value v ->
+    t --[e]--> t' ->
+    <{ v = t }> --[e]--> <{ v = t' }>
+
+  | TS_Asg : forall ad v T,
+    value v ->
+    <{ &ad :: T = v }> --[EF_Write ad v T]--> <{ unit }>
+
+  (* Call *)
+  | TS_Call1 : forall t1 t1' t2 e,
+    t1 --[e]--> t1' ->
+    <{ call t1 t2 }> --[e]--> <{ call t1' t2 }>
+
+  | TS_Call2 : forall t t' v e,
+    value v ->
+    t --[e]--> t' ->
+    <{ call v t }> --[e]--> <{ call v t' }>
+
+  | TS_Call : forall x Tx t v,
+    value v ->
+    <{ call <{ fn x Tx t }> v }> --[EF_None]--> ([x := v] t)
+
+  (* Seq *)
+  | TS_Seq1 : forall t1 t1' t2 e,
+    t1 --[e]--> t1' ->
+    <{ t1; t2 }> --[e]--> <{ t1'; t2 }>
+
+  | TS_Seq : forall v t,
+    value v ->
+    <{ v; t }> --[EF_None]--> t
+
+  (* Spawn *)
+  | TS_Spawn : forall t,
+    <{ spawn t }> --[EF_Spawn t]--> <{ unit }>
+
+  where "t '--[' e ']-->' t'" := (tstep t e t').
+
+(* ------------------------------------------------------------------------- *)
+(* operational semantics -- memory step                                      *)
+(* ------------------------------------------------------------------------- *)
+
+Definition mem := list (tm * typ).
+Definition memory_default := (<{ unit }>, <{{ Unit }}>).
+
+Notation " l '[' i '].tm' " := (fst (l[i] or memory_default))
+  (at level 9, i at next level).
+Notation " l '[' i '].typ' " := (snd (l[i] or memory_default))
+  (at level 9, i at next level).
+
+Inductive mstep : mem -> tm -> eff -> mem -> tm -> Prop :=
+  | MS_Alloc : forall m t t' ad v T,
+    ad = #m ->
+    t --[EF_Alloc ad v T]--> t' ->
+    m / t ==[EF_Alloc ad v T]==> (m +++ (v, T)) / t'
+
+  | MS_Read : forall m t t' ad,
+    ad < #m ->
+    t --[EF_Read ad m[ad].tm]--> t' ->
+    m / t ==[EF_Read ad m[ad].tm]==> m / t'
+
+  | MS_Write : forall m t t' ad v T,
+    ad < #m ->
+    t --[EF_Write ad v T]--> t' ->
+    m / t ==[EF_Write ad v T]==> m[ad <- (v, T)] / t'
+
+  | MS_None : forall m t t',
+    t --[EF_None]--> t' ->
+    m / t ==[EF_None]==> m / t'
+
+  where "m / t '==[' e ']==>' m' / t'" := (mstep m t e m' t').
+
+(* ------------------------------------------------------------------------- *)
+(* operational semantics -- concurrent step                                  *)
+(* ------------------------------------------------------------------------- *)
+
+Definition threads := list tm.
+Definition thread_default := <{ unit }>.
+Definition thread_id := nat.
+
+Notation " l '[' i ']' " := (l[i] or thread_default)
+  (at level 9, i at next level).
+
+Inductive cstep :
+  mem -> threads -> thread_id -> eff -> mem -> threads -> Prop :=
+
+  | CS_Spawn : forall m t' ths tid block,
+      tid < #ths ->
+      ths[tid] --[EF_Spawn block]--> t' ->
+      m / ths ~~[tid, EF_Spawn block]~~> m / (ths[tid <- t'] +++ block)
+
+  | CS_Mem : forall m m' t' ths tid e,
+      tid < #ths ->
+      m / ths[tid] ==[e]==> m' / t' ->
+      m / ths ~~[tid, e]~~> m' / ths[tid <- t']
+
+  where "m / ths '~~[' tid ,  e ']~~>' m' / ths'" :=
+    (cstep m ths tid e m' ths').
+
+(* ------------------------------------------------------------------------- *)
+(* multistep                                                                 *)
+(* ------------------------------------------------------------------------- *)
+
+Definition trace := list (thread_id * eff).
+
+Inductive multistep : mem -> threads -> trace -> mem -> threads -> Prop :=
+  | multistep_refl: forall m ths,
+    m / ths ~~[nil]~~>* m / ths
+
+  | multistep_trans : forall m m' m'' ths ths' ths'' tc tid e,
+    m  / ths  ~~[tc]~~>* m'  / ths'  ->
+    m' / ths' ~~[tid, e]~~> m'' / ths'' ->
+    m  / ths  ~~[(tid, e) :: tc]~~>* m'' / ths''
+
+  where "m / t '~~[' tc ']~~>*' m' / t'" := (multistep m t tc m' t').
+
