Makefile
@@ -2,38 +2,35 @@
 
 COQC= coqc -Q . Elo
 
-all: core meta definitions properties soundness safety
+all: core meta properties preservation soundness safety
 
 core:
 	$(COQC) Util.v
 	$(COQC) Array.v
 	$(COQC) Map.v
+	$(COQC) Sem.v
+	$(COQC) Ext.v
 	$(COQC) Core.v
-	$(COQC) CoreExt.v
 
 meta:
-	$(COQC) AnyTerm.v
 	$(COQC) Meta.v
 
-definitions:
-	$(COQC) ValidAddresses.v
-	$(COQC) WellTypedTerm.v
-	$(COQC) CTR.v
-	$(COQC) Access.v
-	$(COQC) UnsafeAccess.v
-	$(COQC) SafeSpawns.v
-	$(COQC) SMS.v
-	$(COQC) Definitions.v
-	$(COQC) Sanity.v
-
 properties:
-	$(COQC) MemTyp.v
-	$(COQC) PropertiesVAD.v
-	$(COQC) PropertiesCTR.v
-	$(COQC) PropertiesACC.v
-	$(COQC) PropertiesUACC.v
-	$(COQC) PropertiesSS.v
-	$(COQC) PropertiesSMS.v
+	$(COQC) Definitions.v
+	$(COQC) Inversions.v
+	$(COQC) Constructors.v
+	$(COQC) Properties.v
+
+preservation:
+	$(COQC) PtrTyp.v
+	$(COQC) Lemmas.v
+	$(COQC) Inheritance.v
+	$(COQC) Preservation.v
+
+# $(COQC) PropertiesVAD.v
+# $(COQC) PropertiesACC.v
+# $(COQC) PropertiesUACC.v
+# $(COQC) PropertiesSS.v
 
 soundness:
 	$(COQC) Soundness.v
